Source/DafnyCompilers/Semantics.dfy
@@ -1,6 +1,8 @@
 include "CompilerCommon.dfy"
+include "Library.dfy"
 
 module Values {
+  import opened Lib.Datatypes
   import Ty = DafnyCompilerCommon.AST.Type
 
   datatype T =
@@ -11,11 +13,11 @@ module Values {
     | BigOrdinal(o: ORDINAL)
     | BitVector(value: int)
     | Map(m: map<T, T>)
-    | Multiset(ms: multiset<T>)
+    | MultiSet(ms: multiset<T>)
     | Seq(sq: seq<T>)
     | Set(st: set<T>)
   {
-    predicate HasType(ty: Ty.Type) {
+    predicate method HasType(ty: Ty.Type) {
       match (this, ty) // FIXME tests on other side
         case (Bool(b), Bool()) => true
         case (Char(c), Char()) => true
@@ -26,13 +28,29 @@ module Values {
           0 <= value < Pow2(width)
         case (Map(m), Collection(true, Map(kT), eT)) =>
           forall x | x in m :: x.HasType(kT) && m[x].HasType(eT)
-        case (Multiset(ms), Collection(true, Multiset, eT)) =>
+        case (MultiSet(ms), Collection(true, MultiSet, eT)) =>
           forall x | x in ms :: x.HasType(eT)
         case (Seq(sq), Collection(true, Seq, eT)) =>
           forall x | x in sq :: x.HasType(eT)
         case (Set(st), Collection(true, Set, eT)) =>
           forall x | x in st :: x.HasType(eT)
-        case (_, _) => false
+
+        case (Bool(b), _) => false
+        case (Char(c), _) => false
+        case (Int(i), _) => false
+        case (Real(r), _) => false
+        case (BigOrdinal(o), _) => false
+        case (BitVector(value), _) => false
+        case (Map(m), _) => false
+        case (MultiSet(ms), _) => false
+        case (Seq(sq), _) => false
+        case (Set(st), _) => false
+    }
+
+    function method Cast(ty: Ty.Type) : (v: Option<T>)
+      ensures v.Some? ==> HasType(ty)
+    {
+      if HasType(ty) then Some(this) else None
     }
   }
 
@@ -43,19 +61,17 @@ module Values {
   }
 
   // FIXME how do we define the interpreter to support :| without committing to a single interpretation of :|?
+  // NOTE: Maybe tag each syntactic :| with a distinct color and add the color somehow into the Dafny-side :| used to implement it.  Pro: it allows inlining.
 }
 
 module Interp {
+  import opened Lib.Datatypes
   import opened DafnyCompilerCommon.AST
   import opened DafnyCompilerCommon.Predicates
-  type Expr = AST.Expr.Expr
+  type Expr = Expr
   type Type = AST.Type.Type
   import V = Values
-  // FIXME reduce indirection
-
-  datatype Result =
-    | OK(v: V.Value)
-    | TypeError(e: Expr, t: Type) // FIXME rule out type errors through Wf predicate
+  // DISCUSS reduce indirection
 
   predicate method Pure1(e: Expr) {
     match e {
@@ -96,13 +112,20 @@ module Interp {
           case FunctionCall() => FALSE
         }
       case Block(stmts: seq<Expr>) => false
-      case If(cond: Expr, thn: Expr, els: Expr) => FALSE
+      case If(cond: Expr, thn: Expr, els: Expr) => true
       case Unsupported(_) => false
     }
   }
 
   predicate method SupportsInterp(e: Expr) {
     Predicates.Deep.All_Expr(e, SupportsInterp1)
+  }
+
+  lemma SupportsInterp_Pure(e: Expr)
+    requires SupportsInterp1(e)
+    ensures Pure1(e)
+  {
+
   }
 
   function method InterpLiteral(a: AST.Expr.Literal) : V.T {
@@ -115,19 +138,270 @@ module Interp {
         V.Seq(seq(|s|, i requires 0 <= i < |s| => V.Char(s[i])))
   }
 
-  type Ctx = map<string, V.Value>
+  type Context = map<string, V.Value> // FIXME V.T or Value?
 
-  function method InterpExpr(e: AST.Expr.Expr, ctx: Ctx := map[]) : (Ctx, V.T)
+  datatype InterpError =
+    | TypeError(e: Expr, value: V.T, expected: Type) // TODO rule out type errors through Wf predicate?
+    | InvalidExpression(e: Expr) // TODO rule out in Wf predicate?
+    | Unsupported(e: Expr) // TODO rule out in SupportsExpr predicate
+    | Overflow(x: int, low: int, high: int)
+    | DivisionByZero
+
+  datatype InterpSuccess<A> =
+    | OK(v: A, ctx: Context)
+
+  type InterpResult<A> =
+    Result<InterpSuccess<A>, InterpError>
+
+  type PureInterpResult<A> =
+    Result<A, InterpError>
+
+  function method LiftPureResult<A>(ctx: Context, r: PureInterpResult<A>) : InterpResult<A> {
+    var v :- r;
+    Success(OK(v, ctx))
+  }
+
+  function method InterpExpr(e: Expr, ctx: Context := map[]) : InterpResult<V.T>
     requires SupportsInterp(e)
+    decreases e, 0
   {
+    Predicates.AllImpliesChildren(e, SupportsInterp1); // DISCUSS
     match e {
-      case Literal(lit) => (ctx, InterpLiteral(lit))
+      case Literal(lit) => Success(OK(InterpLiteral(lit), ctx))
       case Apply(aop, args: seq<Expr>) =>
+        // FIXME short-circuiting operators should be separate
+        var OK(argsv, ctx) :- InterpExprs(args, ctx);
         match aop {
-          case UnaryOp(uop: UnaryOp.Op) => (ctx, V.Int(0))
-          case BinaryOp(bop: BinaryOp.Op) => (ctx, V.Int(0))
+          case BinaryOp(bop: BinaryOp.Op) =>
+            assert |argsv| == 2;
+            LiftPureResult(ctx, InterpBinaryOp(e, bop, argsv[0], argsv[1]))
         }
-      case If(_, _, _) => assert false; (ctx, V.Int(0))
+      case If(cond, thn, els) =>
+        var OK(condv, ctx) :- InterExprWithType(cond, Type.Bool, ctx);
+        if condv.b then InterpExpr(thn, ctx) else InterpExpr(els, ctx)
     }
+  }
+
+  function method InterExprWithType(e: Expr, ty: Type, ctx: Context := map[]) : (r: InterpResult<V.T>)
+    requires SupportsInterp(e)
+    decreases e, 1
+    ensures r.Success? ==> r.value.v.HasType(ty)
+  {
+    var OK(val, ctx) :- InterpExpr(e, ctx);
+    :- Need(val.HasType(ty), TypeError(e, val, ty));
+    Success(OK(val, ctx))
+  }
+
+  function method InterpExprs(es: seq<Expr>, ctx: Context) : (r: InterpResult<seq<V.T>>)
+    requires forall e | e in es :: SupportsInterp(e)
+    ensures r.Success? ==> |r.value.v| == |es|
+  {
+    if es == [] then Success(OK([], ctx))
+    else
+      var OK(v, ctx) :- InterpExpr(es[0], ctx);
+      var OK(vs, ctx) :- InterpExprs(es[1..], ctx);
+      Success(OK([v] + vs, ctx))
+  }
+
+  function method InterpBinaryOp(expr: Expr, bop: AST.BinaryOp.Op, v0: V.T, v1: V.T) : PureInterpResult<V.T> {
+    match bop
+      case Numeric(op) => InterpNumeric(expr, op, v0, v1)
+      case Logical(op) => InterpLogical(expr, op, v0, v1)
+      case Eq(op) => match op { // FIXME which types is this Eq applicable to (vs. the type-specific ones?)
+        case EqCommon => Success(V.Bool(v0 == v1))
+        case NeqCommon => Success(V.Bool(v0 != v1))
+      }
+      case BV(op) => Failure(Unsupported(expr))
+      case Char(op) => InterpChar(expr, op, v0, v1)
+      case Sets(op) => InterpSets(expr, op, v0, v1)
+      case MultiSets(op) => InterpMultiSets(expr, op, v0, v1)
+      case Sequences(op) => InterpSequences(expr, op, v0, v1)
+      case Maps(op) => InterpMaps(expr, op, v0, v1)
+      case Datatypes(op) => Failure(Unsupported(expr))
+
+  }
+
+  function method InterpNumeric(expr: Expr, op: BinaryOp.Numeric, v0: V.T, v1: V.T) : PureInterpResult<V.T> {
+    match (v0, v1) {
+      // Separate functions to more easily check exhaustiveness
+      case (Int(x1), Int(x2)) => InterpInt(expr, op, x1, x2)
+      case (Char(x1), Char(x2)) => InterpNumericChar(expr, op, x1, x2)
+      case (Real(x1), Real(x2)) => InterpReal(expr, op, x1, x2)
+      case _ => Failure(InvalidExpression(expr)) // FIXME: Wf
+    }
+  }
+
+  function method CheckDivisionByZero(b: bool) : Outcome<InterpError> {
+    if b then Fail(DivisionByZero) else Pass
+  }
+
+  function method InterpInt(expr: Expr, bop: AST.BinaryOp.Numeric, x1: int, x2: int) : PureInterpResult<V.T> {
+    match bop {
+      case Lt() => Success(V.Bool(x1 < x2))
+      case Le() => Success(V.Bool(x1 <= x2))
+      case Ge() => Success(V.Bool(x1 >= x2))
+      case Gt() => Success(V.Bool(x1 > x2))
+      case Add() => Success(V.Int(x1 + x2))
+      case Sub() => Success(V.Int(x1 - x2))
+      case Mul() => Success(V.Int(x1 * x2))
+      case Div() => :- CheckDivisionByZero(x2 == 0); Success(V.Int(x1 / x2))
+      case Mod() => :- CheckDivisionByZero(x2 == 0); Success(V.Int(x1 % x2))
+    }
+  }
+
+  function method CheckOverflow(x: int, low: int, high: int) : PureInterpResult<int> {
+    if low <= x < high then Success(x) else Failure(Overflow(x, low, high))
+  }
+
+  function method InterpNumericChar(expr: Expr, bop: AST.BinaryOp.Numeric, x1: char, x2: char) : PureInterpResult<V.T> {
+    match bop { // FIXME: These first four cases are not used (see InterpChar instead)
+      case Lt() => Success(V.Bool(x1 < x2))
+      case Le() => Success(V.Bool(x1 <= x2))
+      case Ge() => Success(V.Bool(x1 >= x2))
+      case Gt() => Success(V.Bool(x1 > x2))
+      case Add() => var x :- CheckOverflow(x1 as int + x2 as int, 0, 256); Success(V.Char(x as char))
+      case Sub() => var x :- CheckOverflow(x1 as int - x2 as int, 0, 256); Success(V.Char(x as char))
+      case Mul() => Failure(Unsupported(expr))
+      case Div() => Failure(Unsupported(expr))
+      case Mod() => Failure(Unsupported(expr))
+    }
+  }
+
+  function method InterpReal(expr: Expr, bop: AST.BinaryOp.Numeric, x1: real, x2: real) : PureInterpResult<V.T> {
+    match bop {
+      case Lt() => Success(V.Bool(x1 < x2))
+      case Le() => Success(V.Bool(x1 <= x2))
+      case Ge() => Success(V.Bool(x1 >= x2))
+      case Gt() => Success(V.Bool(x1 > x2))
+      case Add() => Success(V.Real(x1 + x2))
+      case Sub() => Success(V.Real(x1 - x2))
+      case Mul() => Success(V.Real(x1 * x2))
+      case Div() => :- CheckDivisionByZero(x2 == 0 as real); Success(V.Real(x1 / x2))
+      case Mod() => Failure(Unsupported(expr))
+    }
+  }
+
+  function method InterpLogical(expr: Expr, op: BinaryOp.Logical, v0: V.T, v1: V.T) : PureInterpResult<V.T> {
+    match (v0, v1) {
+      case (Bool(b1), Bool(b2)) =>
+        match op {
+          case Iff() => Success(V.Bool(b1 <==> b2))
+          case Or() => Failure(Unsupported(expr)) // FIXME move to top-level AST
+          case And() => Failure(Unsupported(expr)) // FIXME move to top-level AST
+          case Imp() => Failure(Unsupported(expr)) // FIXME move to top-level AST
+        }
+      case _ => Failure(InvalidExpression(expr)) // FIXME: Wf
+    }
+  }
+
+  function method InterpChar(expr: Expr, op: AST.BinaryOp.Char, v0: V.T, v1: V.T) : PureInterpResult<V.T> { // FIXME eliminate distinction between GtChar and GT?
+    match (v0, v1) {
+      case (Char(x1), Char(x2)) =>
+        match op {
+          case LtChar() => Success(V.Bool(x1 < x2))
+          case LeChar() => Success(V.Bool(x1 <= x2))
+          case GeChar() => Success(V.Bool(x1 >= x2))
+          case GtChar() => Success(V.Bool(x1 > x2))
+        }
+      case _ => Failure(InvalidExpression(expr)) // FIXME: Wf
+    }
+  }
+
+  function method InterpSets(expr: Expr, op: BinaryOp.Sets, v0: V.T, v1: V.T) : PureInterpResult<V.T> {
+    match (v0, v1)
+      case (Set(s0), Set(s1)) =>
+        match op {
+          case SetEq => Success(V.Bool(s0 == s1))
+          case SetNeq => Success(V.Bool(s0 != s1))
+          case Subset => Success(V.Bool(s0 <= s1))
+          case Superset => Success(V.Bool(s0 >= s1))
+          case ProperSubset => Success(V.Bool(s0 < s1))
+          case ProperSuperset => Success(V.Bool(s0 > s1))
+          case Disjoint => Success(V.Bool(s0 !! s1))
+          case Union => Success(V.Set(s0 + s1))
+          case Intersection => Success(V.Set(s0 * s1))
+          case SetDifference => Success(V.Set(s0 - s1))
+          case InSet => Failure(InvalidExpression(expr))
+          case NotInSet => Failure(InvalidExpression(expr))
+        }
+      case (_, Set(s1)) =>
+        match op {
+          case InSet => Success(V.Bool(v0 in s1))
+          case NotInSet => Success(V.Bool(v0 !in s1))
+          case _ => Failure(InvalidExpression(expr))
+        }
+      case _ => Failure(InvalidExpression(expr))
+  }
+
+  function method InterpMultiSets(expr: Expr, op: BinaryOp.MultiSets, v0: V.T, v1: V.T) : PureInterpResult<V.T> {
+    match (v0, v1)
+      case (MultiSet(m0), MultiSet(m1)) =>
+        match op {
+          case MultiSetEq => Success(V.Bool(m0 == m1))
+          case MultiSetNeq => Success(V.Bool(m0 != m1))
+          case MultiSubset => Success(V.Bool(m0 <= m1))
+          case MultiSuperset => Success(V.Bool(m0 >= m1))
+          case ProperMultiSubset => Success(V.Bool(m0 < m1))
+          case ProperMultiSuperset => Success(V.Bool(m0 > m1))
+          case MultiSetDisjoint => Success(V.Bool(m0 !! m1))
+          case MultiSetUnion => Success(V.MultiSet(m0 + m1))
+          case MultiSetIntersection => Success(V.MultiSet(m0 * m1))
+          case MultiSetDifference => Success(V.MultiSet(m0 - m1))
+          case InMultiSet => Failure(InvalidExpression(expr))
+          case NotInMultiSet => Failure(InvalidExpression(expr))
+        }
+      case (_, MultiSet(s1)) =>
+        match op {
+          case InMultiSet => Success(V.Bool(v0 in s1))
+          case NotInMultiSet => Success(V.Bool(v0 !in s1))
+          case _ => Failure(InvalidExpression(expr))
+        }
+      case _ => Failure(InvalidExpression(expr))
+  }
+
+  function method InterpSequences(expr: Expr, op: BinaryOp.Sequences, v0: V.T, v1: V.T) : PureInterpResult<V.T> {
+    match (v0, v1)
+      case (Seq(s0), Seq(s1)) =>
+        match op {
+          case SeqEq => Success(V.Bool(s0 == s1))
+          case SeqNeq => Success(V.Bool(s0 != s1))
+          case Prefix => Success(V.Bool(s0 <= s1))
+          case ProperPrefix => Success(V.Bool(s0 < s1))
+          case Concat => Success(V.Seq(s0 + s1))
+          case InSeq => Failure(InvalidExpression(expr))
+          case NotInSeq => Failure(InvalidExpression(expr))
+        }
+      case (_, Seq(s1)) =>
+        match op {
+          case InSeq => Success(V.Bool(v0 in s1))
+          case NotInSeq => Success(V.Bool(v0 !in s1))
+          case _ => Failure(InvalidExpression(expr))
+        }
+      case _ => Failure(InvalidExpression(expr))
+  }
+
+  function method InterpMaps(expr: Expr, op: BinaryOp.Maps, v0: V.T, v1: V.T) : PureInterpResult<V.T> {
+    match (v0, v1)
+      case (Map(m0), Map(m1)) =>
+        match op {
+          case MapEq => Success(V.Bool(m0 == m1))
+          case MapNeq => Success(V.Bool(m0 != m1))
+          case MapMerge => Success(V.Map(m0 + m1))
+          case MapSubtraction => Failure(InvalidExpression(expr))
+          case InMap => Failure(InvalidExpression(expr))
+          case NotInMap => Failure(InvalidExpression(expr))
+        }
+      case (Map(m0), Set(s1)) =>
+        match op {
+          case MapSubtraction => Success(V.Map(m0 - s1))
+          case _ => Failure(InvalidExpression(expr))
+        }
+      case (_, Map(m1)) =>
+        match op {
+          case InMap => Success(V.Bool(v0 in m1))
+          case NotInMap => Success(V.Bool(v0 !in m1))
+          case _ => Failure(InvalidExpression(expr))
+        }
+      case _ => Failure(InvalidExpression(expr))
   }
 }
