Source/DafnyCompilers/Printer.dfy
@@ -12,11 +12,11 @@ module Interp.Printer {
       case Bool(b) => Str.of_bool(b)
       case Char(c) => Str.of_char(c)
       case Int(i) => Str.of_int(i)
-      case Real(r) => var (n, d) := Interop.Reals.AsIntegerRatio(r); Str.of_int(n) + "/" + Str.of_int(d)
+      case Real(r) => var (n, d) := Interop.TypeConv.AsIntegerRatio(r); Str.of_int(n) + "/" + Str.of_int(d)
       case BigOrdinal(o) => "<*>" // FIXME
       case BitVector(value) => "bv(" + Str.of_int(value, 16) + ")"
       case Map(m) => "map[" + "<*>" + "]" // FIXME iterate over map
-      case Multiset(ms) => "multiset{" + "<*>" + "}]" // FIXME iterate over multiset (convert to map?)
+      case MultiSet(ms) => "multiset{" + "<*>" + "}]" // FIXME iterate over multiset (convert to map?)
       case Seq(sq) => "[" + Lib.Str.Join(",", Lib.Seq.Map(v requires v in sq => ToString(v), sq)) + "]"
       case Set(st) => "set{" + "<*>" + "}" // FIXME iterate over set
   }
